backends/lean/Aeneas/Std/Array/Core.lean
@@ -34,10 +34,14 @@ theorem List.mapM_clone_eq {T : Type u} {clone : T → Result T} {l : List T}
   apply h
 
 def List.clone (clone : α → Result α) (l : List α) : Result ({ l' : List α // l'.length = l.length}) :=
-  match h :List.mapM clone l with
-  | ok v => ok ⟨ v, by have := List.mapM_Result_length h; scalar_tac ⟩
-  | fail e => fail e
-  | div => div
+  -- match h :List.mapM clone l with
+  -- | ok v => ok ⟨ v, by have := List.mapM_Result_length h; scalar_tac ⟩
+  -- | fail e => fail e
+  -- | div => div
+  (List.mapM clone l).match
+  (fun v => ok ⟨ v, by have := List.mapM_Result_length h; scalar_tac ⟩)
+  (fun e => fail e)
+  div
 
 @[step]
 def List.clone_spec {clone : α → Result α} {l : List α} (h : ∀ x ∈ l, clone x = ok x) :
